Ntt spec and implementation equivalence; carries missing

proof/correctness/R256.ec
@@ -22,13 +22,12 @@ clone include PolyQPrincipalIdeal
 
 end R256.
 
+export R256.
+
 theory KyberPoly.
 
-clone import R256.
 import Fq.
 import ZModP.
-
-type elem = W16.t.
 
 op q = W16.of_int 3329 axiomatized by qE.
 
@@ -47,8 +46,8 @@ lemma add_corr (a b : W16.t) (a' b' : zmod) (asz bsz : int):
      inzmod (W16.to_sint (add a b)) = a' + b' /\
            bw16 (add a b) (max asz bsz + 1).
 admitted.
-(* slow 
-proof
+(* slow
+proof.
 rewrite /bw16 /add !to_sintE !_smodE => />.
 move => ?? ?? [#?] ?? [#?] ??.
 
@@ -117,7 +116,12 @@ require import NTT_Fq.
 clone import NTT_Fq with
    op ZModP.p <- Fq.q,
    type ZModP.zmod <- zmod,
-   theory ZModP.Sub <- Sub,
+   op ZModP.zero  <- Fq.ZModP.zero,
+   op ZModP.one   <- Fq.ZModP.one  ,
+   op ZModP.( + )  <- Fq.ZModP.( + ),
+   op ZModP.([-])  <- Fq.ZModP.([-]),
+   op ZModP.( * )  <- Fq.ZModP.( * ),
+   op ZModP.inv   <- Fq.ZModP.inv  ,
    op ZModP.inzmod <- inzmod,
    op ZModP.asint <- asint. (* .. *)
 
@@ -128,6 +132,7 @@ require import Array256.
 import Fq.SignedReductions.
 
 print M.
+
 lemma poly_reduct_corr:
     forall (_a : int Array256.t),
       phoare[ M.poly_reduce :
@@ -159,6 +164,9 @@ qed.
 op lift_array (p : W16.t Array256.t) =
   Array256.map (fun x => inzmod (W16.to_sint x)) p.
 
+op lift_array_mont (p : W16.t Array256.t) =
+  Array256.map (fun x => inzmod (W16.to_sint x) *  (inzmod 169)) p. (* we cancel the Mont rep *)
+
 op load_array_from_mem(mem : global_mem_t, ptr : W64.t) : W16.t Array256.t.
 
 axiom load_array_from_memE mem ptr i :
@@ -169,15 +177,15 @@ print NTT_Fq.NTT.
 print lift_array_from_mem.
 equiv ntt_correct &m :
   NTT_Fq.NTT.ntt ~ M.poly_ntt : 
+        to_uint zetasp{2}  < W64.modulus - 514 /\
         r{1} = lift_array rp{2} /\ 
-        zetas{1} = lift_array (load_array_from_mem Glob.mem{2} zetasp{2}) ==> 
+        zetas{1} = lift_array_mont (load_array_from_mem Glob.mem{2} zetasp{2}) ==> 
             res{1} = lift_array res{2} /\
             all (fun x => 0<= W16.to_sint x < 2*Fq.q) res{2}.
 proc.
 seq 3 2 : 
     (forall k, 0 <= k < 256 => 
-       (-32768 < to_sint rp{2}.[k] < 32768 /\
-       r{1} = lift_array rp{2})); last first.
+       r{1} = lift_array rp{2}); last first.
 exists * r{1}, rp{2}.
 elim* => r1 rp2.
 call {2} (_:  
@@ -192,16 +200,166 @@ skip. move => &1 &2 [#] ???.
 split.
 move => i ibnd; first by smt (@Array256).
 move => ???.
+have bnds : (
+ forall (k : int),
+      0 <= k < 256 =>
+      -32768 <= to_sint rp{2}.[k] < 32768
+). move => k kb. rewrite to_sintE _smodE => />. 
+   case(32768 <= to_uint rp{2}.[k]); smt.
 split.
 + rewrite (Array256.ext_eq r{1} (lift_array result)) //=.
    move => x xb;rewrite /lift_array  mapiE //=  (H3 x xb) mapiE => />.
    move : (BREDCp_corr (to_sint rp2.[x]) 26 _ _ _ _ _);
       first 5 by smt(@Fq).  
-   move : (H1 x xb);rewrite Array256.tP => [# ] ??? [#] ???.
-   move : (H6 x xb);rewrite /lift_array mapiE => /> *;smt(@ZModP).
+   move : (H1 x xb);rewrite Array256.tP => [# ] ? [#] ???.
+   move : (H4 x xb);rewrite /lift_array mapiE => /> *;smt(@ZModP).
 + rewrite allP => i ib />.  
   rewrite  (H3 i ib) mapiE => />.
   move : (BREDCp_corr (to_sint rp2.[i]) 26 _ _ _ _ _);smt(@Fq @ZModP).
-admitted.
+sp.
+exists *zetasp{2}.
+elim* => zetasp2.
+while (
+   to_uint zetasp{2} + 512 - (k{1}-1)*2 < W64.modulus /\
+   r{1} = lift_array rp{2} /\
+   zetas{1} = lift_array_mont 
+              (load_array_from_mem Glob.mem{2} zetasp2) /\
+   len{1} = to_uint len{2} /\
+   1 <= len{1} <= 128 /\
+   1 <= k{1} <= 256 /\
+   to_uint zetasp{2} = to_uint zetasp2 + (k{1}-1)*2 /\
+   2*k{1}*len{1} = 256); last by  auto => />; smt(@W64).
+wp.
+exists* k{1}.
+elim* => k1.
+while (#{/~k1=k{1}}
+        {~2*k{1}*len{1} = 256}pre /\ 
+       2*k1*len{1}= 256 /\
+       start{1} = to_uint start{2} /\
+       0 <= start{1} <= 256 /\
+       start{1} = 2*(k{1} - k1)*len{1}); last by
+ auto => />; move => *;rewrite uleE !shr_div; by smt(@W64).
+
+wp.
+while (#{/~start{1} = 2*(k{1} - k1) * len{1}}pre /\
+       zeta_{1} = inzmod (to_sint zeta_0{2}) *  (inzmod 169) /\  
+       start{1} = 2*((k{1}-1) - k1) * len{1} /\
+       W64.to_uint cmp{2} = start{1} + len{1} /\ 
+       j{1} = to_uint j{2} /\
+       start{1} <= j{1} <= start{1} + len{1});last first. auto => />. 
+move => &1 &2 ??????????????.
+split.
+split; last by rewrite ultE to_uintD_small; by smt(@W64).
+split. 
+split; first by rewrite !to_uintD_small of_uintK => />;smt(@IntExtra @W64).
+split; first by smt(@W64).
+split; last by rewrite to_uintD_small; by smt(@W64). 
+by smt(@W64).
+split. admit.
+split; first by rewrite to_uintD_small; by smt(@W64). 
+by smt(@W64).
+
+move => *.
+split.
+split; first by rewrite !to_uintD_small => />;  by smt(@W64).
+split; last first. 
+rewrite (_:to_uint j_R = to_uint start{2} + to_uint len{2}).
+smt. ring. rewrite H10. by ring.
+split; first   by smt(@W64).
+move => *. 
+rewrite (_:to_uint j_R = to_uint start{2} + to_uint len{2}).
+smt(@W64).  rewrite H10. 
+have stronger : (2*(k{1}+1)*to_uint len{2}  <= 512); smt().
+split.  move => * />. 
+rewrite ultE /of_uingK => />.
+rewrite to_uintD_small. smt(@W64). smt(@W64). 
+rewrite ultE /of_uingK => />.
+rewrite to_uintD_small. smt(@W64). 
+smt(@W64).
+
+wp. sp.
+exists* t{2}, zeta_0{2}.
+elim* => t2 zeta_02.
+call {2} (_:
+   to_sint a = to_sint t2 /\ to_sint b = to_sint zeta_02   
+   ==> 
+  to_sint res = SREDC (to_sint t2 * to_sint zeta_02)
+). apply (fqmul_corr (to_sint t2) (to_sint zeta_02)).
+skip => />.
+move => &1 &2 [#] ?? ?? ?? ?? ?? ?? ?????????.
+split; last by smt(@W64).
+split; last by smt(@W64).
+apply (Array256.ext_eq 
+   ((lift_array rp{2}).[to_uint j{2} + to_uint len{2} <-
+  ((lift_array rp{2}).[to_uint j{2}] + -
+   (inzmod (to_sint zeta_0{2}) * inzmod 169 * (lift_array rp{2}).[to_uint j{2} + to_uint len{2}])%ZModP)%ZModP.ZModpRing].[
+  to_uint j{2} <-
+  ((lift_array rp{2}).[to_uint j{2} + to_uint len{2} <-
+     ((lift_array rp{2}).[to_uint j{2}] + -
+      (inzmod (to_sint zeta_0{2}) * inzmod 169 * (lift_array rp{2}).[to_uint j{2} + to_uint len{2}])%ZModP)%ZModP.ZModpRing].[
+   to_uint j{2}] + inzmod (to_sint zeta_0{2}) * inzmod 169 * (lift_array rp{2}).[to_uint j{2} + to_uint len{2}])%ZModP])
+   (lift_array
+  rp{2}.[to_uint (j{2} + len{2}) <- rp{2}.[to_uint j{2}] - result].[to_uint j{2} <- result + rp{2}.[to_uint j{2}]])
+).
+
+have to_sintD_small : (forall (a b : W16.t), 
+    -W16.modulus %/2 <= to_sint a + to_sint b < W16.modulus %/2 =>
+    to_sint (a + b) = to_sint a + to_sint b).
+  move => a b.
+  rewrite !W16.to_sintE !_smodE => />.  admit.
+
+have to_sintB_small : (forall (a b : W16.t), 
+    -W16.modulus %/2 <= to_sint a - to_sint b < W16.modulus %/2 =>
+    to_sint (a - b) = to_sint a - to_sint b).
+  move => a b.
+  rewrite !W16.to_sintE !_smodE => />.  admit.
+
+have to_sintM_small : (forall (a b : W16.t), 
+    -W16.modulus %/2 <= to_sint a * to_sint b < W16.modulus %/2 =>
+    to_sint (a * b) = to_sint a * to_sint b).
+  move => a b.
+  rewrite !W16.to_sintE !_smodE => />.  admit.
+
+move => x xb => />.
+rewrite !to_uintD_small; first by smt(@W64).
+rewrite /lift_array !mapiE => />.   admit. admit.
+
+case (x <> to_uint j{2}). 
+case (x <> to_uint j{2} + to_uint len{2}); first by smt(@Array256).
+
+move => *.
+rewrite Array256.set_neqiE. smt(@W64). smt(@W64).
+rewrite Array256.set_eqiE. smt(@W64). smt(@W64).
+rewrite Array256.set_neqiE. smt(@W64). smt(@W64).
+rewrite Array256.set_eqiE. smt(@W64). smt(@W64).
+rewrite to_sintB_small. admit.
+rewrite H18.
+move : (SREDCp_corr ((to_sint rp{2}.[to_uint (j{2} + len{2})] * to_sint zeta_0{2})) _ _). smt(@Fq). admit.
+rewrite -H18. 
+rewrite !inzmodB.
+move => *.
+rewrite (_: inzmod (to_sint result) = 
+   inzmod (to_sint rp{2}.[to_uint (j{2} + len{2})] * to_sint zeta_0{2} * 169)). smt(@ZModP).
+rewrite !to_uintD_small; first by smt(@W64).
+rewrite !inzmodM. by ring.
+
+case (x <> to_uint j{2} + to_uint len{2}); last by smt(@Array256).
+
+move => *.
+rewrite (_: x = to_uint j{2}); first by smt().
+rewrite Array256.set_eqiE. smt(@W64). smt(@W64).
+rewrite Array256.set_neqiE. admit. smt(@W64).
+rewrite Array256.set_eqiE. smt(@W64). smt(@W64).
+rewrite to_sintD_small. admit.
+rewrite H18 => />.
+move : (SREDCp_corr ((to_sint rp{2}.[to_uint (j{2} + len{2})] * to_sint zeta_0{2})) _ _). smt(@Fq). admit.
+rewrite -H18. 
+rewrite !inzmodD.
+move => *.
+rewrite (_: inzmod (to_sint result) = 
+   inzmod ((to_sint rp{2}.[to_uint (j{2} + len{2})] * to_sint zeta_0{2} * 169))). smt(@ZModP).
+rewrite !to_uintD_small; first by smt(@W64).
+rewrite !inzmodM. ring. smt(@ZModP @Array256).
+qed.
 
 end KyberPoly.
